Prove the barrier except for cancellation

formal-proofs/theories/lib/barrier/barrier.v
@@ -1,6 +1,7 @@
 From iris.heap_lang Require Import notation.
 
 Require Import SegmentQueue.lib.thread_queue.thread_queue.
+Require Import SegmentQueue.lib.thread_queue.thread_queue_as_counter.
 
 Section impl.
 
@@ -31,10 +32,10 @@ Definition cancellation_handler : val :=
        else "loop" "ctr" "head" "deqIdx" "canceller".
 
 Definition await : val :=
-  λ: "threadHandle" "ctr" "tail" "enqIdx" "head" "deqIdx",
+  λ: "cancHandle" "threadHandle" "ctr" "tail" "enqIdx" "head" "deqIdx",
   let: "p" := FAA "ctr" #1
   in if: "p" = #(Pos.to_nat limit-1)
-     then forRange "p" (λ: "i", resume segment_size "head" "deqIdx")
+     then forRange "p" (λ: "i", resume segment_size "head" "deqIdx") ;; #false
      else suspend segment_size (cancellation_handler "ctr" "head" "deqIdx")
                   "cancHandle" "threadHandle" "tail" "enqIdx".
 
@@ -54,25 +55,57 @@ Section proof.
 
 Context `{!heapG Σ}.
 
-Theorem forRange_spec (Φ: nat -> iProp Σ) (e: val):
-  (∀ i, {{{ Φ i }}}
-           e #i
-         {{{ v, RET v; Φ (S i) }}})
+Theorem forRange_spec (Φ: nat -> iProp Σ) (e: val) (n: nat):
+  (∀ i, ⌜(i < n)%nat⌝ -∗ {{{ Φ i }}}
+                           e #i
+                         {{{ v, RET v; Φ (S i) }}})
    -∗
-   (∀ n, {{{ Φ O }}}
-           forRange #n e
-         {{{ v, RET v; Φ n }}}).
+   {{{ Φ O }}}
+     forRange #n e
+   {{{ v, RET v; Φ n }}}.
 Proof.
-  iIntros "#HE" (n Ψ).
+  iIntros "#HE" (Ψ).
   iInduction n as [|n'] "IH" forall (Ψ); iIntros "!> HΦ0 HΨ"; wp_lam; wp_pures.
   by iApply "HΨ".
   replace #(S n' - 1) with #n'; last by congr (fun x => LitV (LitInt x)); lia.
   wp_bind (forRange _ _).
-  wp_apply ("IH" with "HΦ0").
+  wp_apply ("IH" with "[] HΦ0").
+  { iIntros "!>" (i HLt). iApply "HE". iPureIntro. lia. }
   iIntros (v) "HΦn".
   wp_pures.
   replace #(S n' - 1) with #n'; last by congr (fun x => LitV (LitInt x)); lia.
-  by wp_apply ("HE" with "HΦn").
+  wp_apply ("HE" with "[] HΦn"); last done.
+  iPureIntro. lia.
+Qed.
+
+Theorem forRange_resource_map (Φ Ψ: nat -> iProp Σ) (e: val):
+  (∀ (i: nat), {{{ Φ i }}}
+                 e #i
+                 {{{ v, RET v; Ψ i }}})
+    -∗
+  (∀ n, {{{ [∗ list] i ∈ seq 0 n, Φ i }}}
+          forRange #n e
+        {{{ v, RET v; [∗ list] i ∈ seq 0 n, Ψ i }}}).
+Proof.
+  iIntros "#HE" (n Ξ) "!> HΦ HΨ".
+  iApply (forRange_spec
+            (fun j => ([∗ list] i ∈ seq j (n-j), Φ i) ∗
+                   ([∗ list] i ∈ seq 0 j, Ψ i))%I
+            with "[] [HΦ]").
+  - iIntros (i HLt). iIntros "!>" (?) "HPre HPost".
+    replace (seq 0 (S i)) with (seq 0 (i + 1)) by (congr (seq 0); lia).
+    rewrite seq_add /=.
+    destruct (n - i)%nat as [|ni] eqn:X; first by lia.
+    simpl.
+    iDestruct "HPre" as "[[HΦi HΦ] HΨ]".
+    wp_apply ("HE" with "HΦi").
+    iIntros (v) "HΨi".
+    iApply "HPost".
+    replace (n - S i)%nat with ni by lia. iFrame. done.
+  - rewrite Nat.sub_0_r. simpl. iFrame.
+  - iIntros (v) "!> HH".
+    iApply "HΨ".
+    iDestruct "HH" as "[_ $]".
 Qed.
 
 End proof.
@@ -99,17 +132,241 @@ Variable (segment_size: positive).
 Definition barrier_entry_piece γ := own γ (◯ (Some (Cinl 1%positive))).
 Definition barrier_exit_piece γ := own γ (◯ (Some (Cinr 1%positive))).
 
-Definition is_barrier_inv γ (ℓ: loc) (n: nat)
-  (epℓ eℓ dpℓ dℓ: loc) (γa γtq γe γd: gname) :=
-  (∃ l deqFront, own γ (● (Some (Cinl limit))) ∗
-    ℓ ↦ #n ∗ (if decide (n < Pos.to_nat limit)%nat
-              then [∗] replicate n (barrier_entry_piece γ)
-              else True) ∗
-    is_thread_queue (N .@ "tq") Nth segment_size True (barrier_exit_piece γ)
-    γa γtq γe γd eℓ epℓ dℓ dpℓ l deqFront ∗
-    let v := count_matching still_present (drop deqFront l) in
-    (⌜if decide (n < Pos.to_nat limit)%nat then v = n else v = O⌝))%I.
+Definition is_barrier_inv γ (ℓ: loc)
+  (epℓ eℓ dpℓ dℓ: loc) (γa γtq γe γd: gname) (n: nat) :=
+  ((if decide (n < Pos.to_nat limit)%nat then own γ (● (Some (Cinl limit))) else
+      if decide (n = Pos.to_nat limit) then own γ (● (Some (Cinr limit))) else
+        False) ∗
+    ℓ ↦ #n ∗ ([∗] replicate (n `mod` Pos.to_nat limit)%nat (barrier_entry_piece γ)) ∗
+    thread_queue_as_counter (N .@ "tq") Nth segment_size True (barrier_exit_piece γ)
+    γa γtq γe γd eℓ epℓ dℓ dpℓ (n `mod` Pos.to_nat limit)%nat)%I.
 
+Definition is_barrier γ ℓ epℓ eℓ dpℓ dℓ γa γtq γe γd :=
+  inv (N .@ "barrier") (∃ n, is_barrier_inv γ ℓ epℓ eℓ dpℓ dℓ γa γtq γe γd n).
 
+Lemma resume_in_barrier_spec γ p epℓ eℓ dpℓ dℓ γa γtq γe γd:
+  is_barrier γ p epℓ eℓ dpℓ dℓ γa γtq γe γd -∗
+  {{{ awakening_permit γtq }}}
+    (resume segment_size) #dpℓ #dℓ
+  {{{ RET #(); True }}}.
+Proof.
+  iIntros "#HBarInv" (Φ) "!> HAwak HΦ". wp_lam. wp_pures.
+  awp_apply (try_deque_thread_as_counter_spec (N .@ "tq") with "HAwak") without "HΦ".
+  iInv "HBarInv" as (?) "(HAuth & Hl & HPieces & HTq)".
+  iAaccIntro with "HTq".
+  {
+    iIntros "HTq !>".
+    iSplitL; last done.
+    iExists _. iFrame.
+  }
+  iIntros (?) "(_ & HTq & HState)".
+  iDestruct "HState" as "[->|HState]".
+  {
+    iSplitL; first by iExists _; iFrame.
+    iIntros "!> HΦ". wp_pures. by iApply "HΦ".
+  }
+
+  iDestruct "HState" as (? ? ?) "(-> & #[HIsThread HThreadLocs] &
+    [[HResTok #HRendRes]|HNoPerms])".
+  2: {
+    iSplitR "HNoPerms".
+    by iExists _; iFrame.
+    iIntros "!> HΦ". wp_pures.
+    awp_apply (unpark_spec with "HIsThread") without "HΦ".
+    iAaccIntro with "HNoPerms".
+    by iIntros ">HNoPerms !>".
+    iIntros "HPerms !> HΦ". wp_pures. by iApply "HΦ".
+  }
+  {
+    iSplitR "HResTok"; first by iExists _; iFrame.
+    iIntros "!> HΦ". wp_pures.
+
+    awp_apply (thread_queue_as_counter_unpark_spec with
+                   "HRendRes HIsThread HThreadLocs") without "HΦ".
+    iInv "HBarInv" as (?) "(HAuth & Hl & HPieces & HTq)".
+    iCombine "HResTok" "HTq" as "HAacc".
+    iAaccIntro with "HAacc".
+    { iIntros "[$ HTq]". iExists _. by iFrame. }
+    iIntros "HTq". iSplitL.
+    by iExists _; iFrame.
+    iIntros "!> HΦ". wp_pures. by iApply "HΦ".
+  }
+Qed.
+
+Lemma ucmra_cancel_local_update {A: ucmraT} (x: A) `{!Cancelable x}:
+  (x, x) ~l~> (ε, ε).
+Proof.
+  intros n f ? Heq. split; first by apply ucmra_unit_validN.
+  apply (cancelableN x); rewrite /= ucmra_unit_right_id; first done.
+  destruct f as [f'|]; simpl in *.
+  by rewrite ucmra_unit_left_id.
+  by rewrite ucmra_unit_right_id.
+Qed.
+
+Lemma await_spec Nint γi cancHandle γth (threadHandle: loc)
+      γ p epℓ eℓ dpℓ dℓ γa γtq γe γd:
+  is_interrupt_handle Nint γi cancHandle -∗
+  is_thread_handle Nth γth #threadHandle -∗
+  is_barrier γ p epℓ eℓ dpℓ dℓ γa γtq γe γd -∗
+  {{{ thread_doesnt_have_permits γth ∗ barrier_entry_piece γ }}}
+  (await segment_size limit) cancHandle #threadHandle #p #epℓ #eℓ #dpℓ #dℓ
+  {{{ (v: bool), RET #v;
+      ⌜v = false⌝ ∧ thread_doesnt_have_permits γth ∗ barrier_exit_piece γ ∨
+      ⌜v = true⌝ ∧ interrupted γi }}}.
+
+Proof.
+  iIntros "#HIntHandle #HThreadHandle #HBarInv" (Φ) "!> [HNoPerms HEnt] HΦ".
+
+  wp_lam. wp_pures. wp_bind (FAA _ _).
+  iInv "HBarInv" as (n) "(HAuth & Hℓ & HEntries & HTq)" "HClose".
+  destruct (decide (n < Pos.to_nat limit)%nat).
+  2: {
+    destruct (decide (n = Pos.to_nat limit)); last by iDestruct "HAuth" as ">[]".
+    iDestruct "HAuth" as ">HAuth".
+    iDestruct (own_valid_2 with "HAuth HEnt") as %[HH _]%auth_both_valid.
+    exfalso.
+
+    move: HH. rewrite Some_included. case. by intros; simplify_eq.
+    rewrite csum_included. case; first done. case.
+    by intros (? & ? & _ & HH & _); simplify_eq.
+    by intros (? & ? & HH & _); simplify_eq.
+  }
+
+  wp_faa.
+  replace (n + 1) with (Z.of_nat (S n)) by lia.
+  destruct (decide (n = Pos.to_nat limit - 1)%nat).
+  {
+    replace (n `mod` Pos.to_nat limit)%nat with (n);
+      last by symmetry; rewrite Nat.mod_small_iff; lia.
+    subst.
+    replace (S (_ - _)) with (Pos.to_nat limit) by lia.
+    rewrite /barrier_entry_piece.
+    iAssert (own γ (◯ Some (Cinl limit))) with "[HEnt HEntries]" as "HFrag".
+    {
+      clear.
+      remember (Pos.to_nat limit) as limN.
+      replace limit with (Pos.of_nat limN) by (subst; apply Pos2Nat.id).
+      assert (limN > 0)%nat as HNonZero by lia.
+      clear HeqlimN.
+      iInduction limN as [|limN'] "IH" forall (HNonZero); simpl in *. lia.
+      inversion HNonZero; first done. subst.
+      destruct limN'; first by lia.
+      rewrite /= Nat.sub_0_r.
+      iDestruct "HEntries" as "[HEnt' HRepl]".
+      iSpecialize ("IH" with "[%] HEnt' HRepl"); first lia.
+      replace (Pos.of_nat (S (S limN'))) with
+          (Pos.of_nat 1%nat + Pos.of_nat (S limN'))%positive
+        by rewrite -Nat2Pos.inj_add //.
+      rewrite Cinl_op Some_op auth_frag_op own_op. iFrame.
+    }
+    iMod (own_update_2 with "HAuth HFrag") as "HAuth".
+    { apply auth_update_dealloc, ucmra_cancel_local_update, _. }
+    iMod (own_update with "HAuth") as "[HAuth HFrag]".
+    by apply auth_update_alloc, (alloc_option_local_update (Cinr limit)).
+    iAssert ([∗] replicate (Pos.to_nat limit) (barrier_exit_piece γ))%I
+      with "[HFrag]" as "HExit".
+    {
+      clear.
+      remember (Pos.to_nat limit) as limN.
+      replace limit with (Pos.of_nat limN) by (subst; apply Pos2Nat.id).
+      assert (limN > 0)%nat as HNonZero by lia.
+      clear HeqlimN.
+      iInduction limN as [|limN'] "IH" forall (HNonZero); simpl in *. lia.
+      inversion HNonZero; subst; first by iFrame.
+      replace (Pos.of_nat (S limN')) with
+          (Pos.of_nat 1%nat + Pos.of_nat limN')%positive;
+        last by rewrite -Nat2Pos.inj_add //; lia.
+      rewrite Cinr_op Some_op auth_frag_op own_op.
+      iDestruct "HFrag" as "[$ HFrag]".
+      iApply ("IH" with "[%] [$]").
+      lia.
+    }
+    (* TODO: dequeue (limit - 1) threads. *)
+    remember (Pos.to_nat limit - 1)%nat as sleepers.
+    replace (Pos.to_nat limit) with (S sleepers) by lia.
+    simpl. iDestruct "HExit" as "[HMyExit HWakers]".
+    iAssert (|==> thread_queue_as_counter (N.@"tq") Nth segment_size True
+                  (barrier_exit_piece γ) γa γtq γe γd eℓ epℓ dℓ dpℓ O
+                  ∗ [∗] replicate sleepers (awakening_permit γtq))%I
+      with "[HTq HWakers]" as ">[HTq HAwaken]".
+    {
+      iClear "HIntHandle HThreadHandle HBarInv". clear.
+      iInduction (sleepers) as [|sleepers] "IH"; simpl.
+      by iFrame.
+      iDestruct "HWakers" as "[HWaker HWakers]".
+      iMod (thread_as_counter_register_for_dequeue with "HWaker HTq")
+        as "[$ HTq]"; first by lia.
+      rewrite /= Nat.sub_0_r.
+      iApply ("IH" with "HTq HWakers").
+    }
+    iMod ("HClose" with "[Hℓ HTq HAuth]") as "_".
+    {
+      subst.
+      replace (S (Pos.to_nat limit - 1)%nat) with (Pos.to_nat limit) by lia.
+      iExists _. iFrame "Hℓ".
+      rewrite decide_False; last lia. rewrite decide_True; last lia.
+      iFrame "HAuth".
+      rewrite Nat.mod_same /=; last lia.
+      iFrame.
+    }
+    iModIntro.
+    wp_pures.
+    rewrite bool_decide_eq_true_2; last by congr (fun x => LitV (LitInt x)); lia.
+    wp_pures.
+    wp_apply (forRange_resource_map
+                (fun _ => awakening_permit γtq) (fun _ => True)%I
+             with "[] [HAwaken]").
+    - iIntros (i Ψ) "!> HAwak HPost". wp_pures.
+      wp_apply (resume_in_barrier_spec with "[$] HAwak").
+      iIntros (_). by iApply "HPost".
+    - remember O as n. clear.
+      iInduction sleepers as [|sleepers] "IH" forall (n); first done. simpl.
+      iDestruct "HAwaken" as "[$ HAwaken]".
+      iApply ("IH" with "HAwaken").
+    - iIntros (v) "_". wp_pures.
+      iApply "HΦ". iLeft. by iFrame.
+  }
+  {
+    iMod (thread_queue_as_counter_append with "[] HTq") as "[HSusp HTq]";
+      first done.
+    iMod ("HClose" with "[-HΦ HSusp HNoPerms]") as "_".
+    {
+      iExists (S n). iFrame "Hℓ".
+      destruct (decide (S n < Pos.to_nat limit)%nat); try lia.
+      iFrame "HAuth".
+      replace (S n `mod` Pos.to_nat limit)%nat with (S n);
+        last by symmetry; rewrite Nat.mod_small_iff; lia.
+      replace (n `mod` Pos.to_nat limit)%nat with (n);
+        last by symmetry; rewrite Nat.mod_small_iff; lia.
+      simpl. iFrame.
+    }
+    iIntros "!>". wp_pures.
+    rewrite bool_decide_eq_false_2.
+    2: intros HContra; inversion HContra; lia.
+    wp_pures.
+
+    wp_lam. wp_pures. wp_lam. wp_pures.
+    awp_apply (try_enque_thread_as_counter_spec (N.@"tq") with
+                   "HThreadHandle HSusp HNoPerms") without "HΦ".
+
+    iInv "HBarInv" as (n') "(HAuth & Hℓ & HEntries & HTq)".
+    iAaccIntro with "HTq".
+    { iIntros "HTq !>". iSplitL; last done. iExists _. iFrame. }
+    iIntros (v) "[HTq HStates]".
+    iIntros "!>".
+    iSplitR "HStates".
+    { iExists _. iFrame. }
+    iIntros "HΦ".
+
+    iDestruct "HStates" as "[HPures|(-> & HR & HNoPerms)]".
+    2: { wp_pures. iApply "HΦ". iLeft. by iFrame. }
+    iDestruct "HPures" as (i s ->) "(#HSegLoc & #HRend & HInhToken)".
+    wp_pures. wp_lam. wp_pures.
+    wp_apply (interruptibly_spec _ (inhabitant_token γtq i)
+                                   (fun _ => thread_has_permit γth ∗ barrier_exit_piece γ)%I
+                                   (fun _ => interrupted γi)
+              with "[HInhToken]").
+
+Abort.
 
 End barrier_proof.
